LeanSorting/Unsafe.lean
@@ -1,0 +1,83 @@
+import Mathlib.Data.Nat.ModEq
+
+@[specialize, inline]
+def mergeAdjacentChunksIntoAuxUnsafe
+    [Ord α]
+    (arr aux : Array α)
+    (start₁ start₂ end₂ : ℕ)
+    : Array α :=
+  let rec @[specialize] loop
+      (aux : Array α)
+      (i k₁ k₂ : ℕ)
+      : Array α :=
+    if k₁ < start₂ ∧ k₂ < end₂ then
+      match Ord.compare (arr[k₁]'sorry) (arr[k₂]'sorry) with
+      | .lt | .eq =>
+        let aux' := aux.set ⟨i, sorry⟩ (arr[k₁]'sorry)
+        loop aux' i.succ k₁.succ k₂
+      | .gt =>
+        let aux' := aux.set ⟨i, sorry⟩ (arr[k₂]'sorry)
+        loop aux' i.succ k₁ k₂.succ
+    else
+      let rec @[specialize] loopLeft
+          (aux : Array α)
+          (i k₁ : ℕ)
+          : Array α :=
+        if k₁ < start₂ then
+          let aux' := aux.set ⟨i, sorry⟩ (arr[k₁]'sorry)
+          loopLeft aux' i.succ k₁.succ
+        else
+          let rec @[specialize] loopRight
+              (aux : Array α)
+              (i k₂ : ℕ)
+              : Array α :=
+            if k₂ < end₂ then
+              let aux' := aux.set ⟨i, sorry⟩ (arr[k₂]'sorry)
+              loopRight aux' i.succ k₂.succ
+            else
+              aux
+          loopRight aux i k₂
+      loopLeft aux i k₁
+  termination_by arr.size - i
+  decreasing_by all_goals sorry
+  loop aux start₁ start₁ start₂
+
+@[specialize, inline]
+def mergeChunksIntoAuxUnsafe
+    [Ord α]
+    (arr aux : Array α)
+    (size : ℕ) :=
+  let rec @[specialize] loop (aux : Array α) (start₁: ℕ)
+      : Array α :=
+    if start₁ + size < arr.size then
+      let start₂ := start₁ + size
+      let end₂ := min (start₂ + size) arr.size
+      let aux' := mergeAdjacentChunksIntoAuxUnsafe arr aux start₁ start₂ end₂
+      loop aux' (start₁ + 2 * size)
+    else
+      let rec @[specialize] loopFinal (aux : Array α) (start₁ : ℕ) : Array α :=
+        if start₁ < aux.size then
+          let aux' := aux.set ⟨start₁, sorry⟩ (arr[start₁]'sorry)
+          loopFinal aux' start₁.succ
+        else
+          aux
+      loopFinal aux start₁
+  termination_by arr.size - start₁
+  decreasing_by sorry
+  loop aux 0
+
+@[specialize]
+def Array.mergeSortUnsafe [Inhabited α] [Ord α] (arr : Array α) : Array α :=
+  let rec @[specialize] loop
+      (arr aux : Array α)
+      (chunkSize : ℕ)
+      : Array α :=
+    if chunkSize < arr.size then
+      let aux' := mergeChunksIntoAuxUnsafe arr aux chunkSize
+      loop aux' arr (chunkSize * 2)
+    else
+      arr
+  termination_by arr.size - chunkSize
+  decreasing_by sorry
+  let aux : Array α := Array.mkArray arr.size default
+  loop arr aux 1
